src/STLC.lean
@@ -1,0 +1,87 @@
+import Init.Data.Nat.Basic
+
+-- We start with a base type and an arrow type --
+inductive typ : Type
+  | base : typ
+  | arrow : typ → typ → typ
+
+-- Conveniance notations --
+notation A"->"B => typ.arrow A B
+
+
+-- We define terms in a recursive manner --
+inductive term : Type
+  | var : Nat → term            -- Each variables is identitifed by a natural number
+  | abs : Nat → term → term     -- Lambda abstraction
+  | app : term → term → term    -- Application
+
+notation "$"n => term.var n
+
+-- We define lists here to be able to embed the context as a list we no duplicates --
+inductive list (T : Type): Type
+  | nil : list T
+  | append : (t : T) → (l : list T) → list T
+
+notation "[]" => list.nil
+notation t","l => list.append t l
+
+inductive in_list (t : T) : list T → Prop
+  | cons : (t = t₀) → in_list t (t₀ , l)
+
+def not_in : T → list T → Prop :=
+  λt => λl => ¬ (in_list t l)
+
+inductive no_duplicates (T : Type) : list T → Prop
+  | nil : no_duplicates T nil
+  | head (t : T) (l : list T): not_in t l → no_duplicates T (t , l)
+
+-- A context is a list of Natural number paired with a type that do not contain duplicates in names --
+structure ctx_elem where
+  name : Nat
+  type : typ
+
+notation "ctx" => list ctx_elem
+-- Carefull, this is "\ :" and not just ":" in the following notation
+notation n"∶"t => ctx_elem.mk n t
+
+def ctx1 : ctx := (3∶typ.base) , []
+
+example : no_duplicates ctx_elem ctx1 := by
+  unfold ctx1
+  apply no_duplicates.head
+  unfold not_in
+  intro p
+  cases p
+
+
+-- We define substitution of the term u for the variable named n in the term t --
+def subst : Nat → term → term → term := by
+  sorry
+
+notation t"[" u "//" n"]" => subst n t u
+
+-- Typing relation --
+inductive TR : ctx → term → typ → Type
+  | var :(n:Nat) → (T : typ) → TR ((n∶T) , []) ($ n) T
+  | abs : (A B : typ) → (n:Nat) → (Γ : ctx ) → (t : term) → TR ((n∶A) , Γ) t B → TR Γ (term.abs n t) (A -> B)
+  | app : (A B : typ) → (Γ : ctx) → (t₀ t₁ : term) →  TR Γ t₀ (A -> B) → TR Γ t₁ A → TR Γ (term.app t₀ t₁) B
+  | sub : (A : typ) → (n:Nat) → (t u : term) → TR Γ t A → TR Γ (t[u // n]) A
+
+notation Γ"⊢"t"∶∶"A => TR Γ t A
+#check ctx1 ⊢ ($ 3) ∶∶ typ.base
+
+example : ctx1 ⊢ ($ 3) ∶∶ typ.base := by
+  apply TR.var
+
+-- We define the beta reduction relation here --
+inductive beta : term → term → Type
+  | cons : beta (term.app (term.abs n t) u) (t[u // n])
+
+-- We prove that betw reduction preserve the typing relation --
+theorem beta_preservation : (A : typ) → (Γ ⊢ t ∶∶ A) → beta t t' → (Γ ⊢ t' ∶∶ A) := by
+  intro A p b
+  induction p
+  case var n T => contradiction
+  case abs B C n Γ₀ t₀ q₀ q₁  => sorry
+  case app B C Γ₀ t₀ t₁ d₀ q₀ q₁ q₂ => sorry
+  case sub B n t₀ u₀ d₀ q₀ q₁ => sorry
